Test/dafny0/Predicates.dfy
@@ -29,3 +29,77 @@ module B refines A {
     }
   }
 }
+
+// ------------------------------------------------
+
+module Loose {
+  class MyNumber {
+    var N: int;
+    ghost var Repr: set<object>;
+    predicate Valid
+      reads this, Repr;
+    {
+      this in Repr && null !in Repr &&
+      0 <= N
+    }
+    constructor Init()
+      modifies this;
+      ensures Valid && fresh(Repr - {this});
+    {
+      N, Repr := 0, {this};
+    }
+    method Inc()
+      requires Valid;
+      modifies Repr;
+      ensures old(N) < N;
+      ensures Valid && fresh(Repr - old(Repr));
+    {
+      N := N + 2;
+    }
+    method Get() returns (n: int)
+      requires Valid;
+      ensures n == N;
+    {
+      n := N;
+    }
+  }
+}
+
+module Tight refines Loose {
+  class MyNumber {
+    predicate Valid
+    {
+      N % 2 == 0
+    }
+    constructor Init()
+      ensures N == 0;
+    method Inc()
+      ensures N == old(N) + 2;
+  }
+}
+
+module UnawareClient imports Loose {
+  class Client {
+    method Main() {
+      var n := new MyNumber.Init();
+      assert n.N == 0;  // error: this is not known
+      n.Inc();
+      n.Inc();
+      var k := n.Get();
+      assert k == 4;  // error: this is not known
+    }
+  }
+}
+
+module AwareClient imports Tight {
+  class Client {
+    method Main() {
+      var n := new MyNumber.Init();
+      assert n.N == 0;
+      n.Inc();
+      n.Inc();
+      var k := n.Get();
+      assert k == 4;
+    }
+  }
+}
